initial commit

src/Std/Data/DTreeMap/Internal/Operations.lean
@@ -485,6 +485,10 @@ def eraseMany! [Ord α] {ρ : Type w} [ForIn Id ρ α] (t : Impl α β) (l : ρ)
 abbrev IteratedInsertionInto [Ord α] (t) :=
   { t' // ∀ {P : Impl α β → Prop}, P t → (∀ t'' a b h, P t'' → P (t''.insert a b h).impl) → P t' }
 
+/-- A tree map obtained by inserting elements into `t` if they are new, bundled with an inductive principle. -/
+abbrev IteratedNewInsertionInto [Ord α] (t) :=
+  { t' // ∀ {P : Impl α β → Prop}, P t → (∀ t'' a b h, P t'' → P (t''.insertIfNew a b h).impl) → P t' }
+
 /-- Iterate over `l` and insert all of its elements into `t`. -/
 @[inline]
 def insertMany [Ord α] {ρ : Type w} [ForIn Id ρ ((a : α) × β a)] (t : Impl α β) (l : ρ) (h : t.Balanced) :
@@ -494,6 +498,17 @@ def insertMany [Ord α] {ρ : Type w} [ForIn Id ρ ((a : α) × β a)] (t : Impl
     let hr := r.2 h (fun t'' a b h _ => (t''.insert a b h).balanced_impl)
     r := ⟨r.val.insert a b hr |>.impl, fun h₀ h₁ => h₁ _ _ _ _ (r.2 h₀ h₁)⟩
   return r
+
+/-- Iterate over `l` and insert all of its elements into `t` if they are new. -/
+@[inline]
+def insertManyIfNew[Ord α] {ρ : Type w} [ForIn Id ρ ((a : α) × β a)] (t : Impl α β) (l : ρ) (h : t.Balanced) :
+    IteratedNewInsertionInto t := Id.run do
+  let mut r := ⟨t, fun h _ => h⟩
+  for ⟨a, b⟩ in l do
+    let hr := r.2 h (fun t'' a b h _ => (t''.insertIfNew a b h).balanced_impl)
+    r := ⟨r.val.insertIfNew a b hr |>.impl, fun h₀ h₁ => h₁ _ _ _ _ (r.2 h₀ h₁)⟩
+  return r
+
 
 /-- A tree map obtained by inserting elements into `t`, bundled with an inductive principle. -/
 abbrev IteratedSlowInsertionInto [Ord α] (t) :=
